environment changes for executabile dec

src/Manifest/Manifest.v
@@ -6,6 +6,7 @@ Import ListNotations.
 Require Import String.
 Require Import Cop.Copland.
 Import Copland.Term.
+Require Import Ltacs TypeClasses Maps.
 
 (** Stuff to do:
  * - Decidability of executable.  Might not work
@@ -40,83 +41,85 @@ Module ManifestTerm.
 *)
     }.
 
+  Theorem asp_dec : forall (a1 a2 : ASP),
+    {a1 = a2} + {a1 <> a2}.
+  Proof.
+    repeat decide equality.
+  Qed.
+
   (** [Environment] is a set of AM's each defined by a [Manifest].
    * The domain of an [Environment] provides names for each [Manifest].
    * Names should be the hash of their public key, but this restriction
    * is not enforced here. 
    *)
 
-  Definition Environment : Type :=  Plc -> (option Manifest).
+  Import MapNotations.
+  Import MapsLtac.
 
-  Definition e_empty : Environment := (fun _ => None).
+  Definition Environment : Type :=  Map Plc Manifest.
+
+  Definition e_empty : Environment := {}.
   
-  Definition e_update (m : Environment) (x : Plc) (v : (option Manifest)) :=
-    fun x' => if plc_dec x x' then v else m x'.
-
+  Definition e_update (m : Environment) (x : Plc) (v : Manifest) :=
+    (x !-> v ; m).
+(* 
   Lemma e_apply_empty: forall x, @e_empty x = None.
   Proof.
     intros.
     auto.
-  Qed.
+  Qed. *)
 
   Lemma e_update_eq : forall (m: Environment) x v,
-      (e_update m x v) x = v.
+      (e_update m x v) ![x] = Some v.
   Proof.
     intros. unfold e_update.
-    case (plc_dec x x).
-    * intro H. reflexivity.
-    * intro H. contradiction.
+    smp. map_unfold. unfold decEq_string.
+    destruct (plc_dec x x); eauto. 
+    cong.
   Qed.
 
   Theorem e_update_neq : forall v x1 x2 (m:Environment),
-      x1 <> x2 -> (e_update m x1 v) x2 = m x2.
+      x1 <> x2 -> (e_update m x1 v) ![x2] = (m ![x2]).
   Proof.
     intros v x1 x2 m.
-    intros H.
-    unfold e_update.
-    case (plc_dec x1 x2); intros H1; [contradiction | reflexivity].
+    intros H. smp.
+    map_unfold. unfold decEq_string.
+    destruct (plc_dec x2 x1); eauto; cong.
   Qed.
 
   Theorem e_update_shadow : forall (m:Environment) v1 v2 x,
-      e_update (e_update m x v1) x v2
-      = e_update m x v2.
+    forall x',
+      (e_update (e_update m x v1) x v2) ![ x'] 
+      = ((e_update m x v2) ![ x']).
   Proof.
-    intros m v1 v2 x.
+    intros m v1 v2 x x'.
     unfold e_update.
-    apply functional_extensionality.
-    intros x0.
-    case (plc_dec x x0).
-    * intros H; reflexivity.
-    * intros H; reflexivity.
+    map_unfold. unfold decEq_string.
+    destruct (plc_dec x' x); eauto.
   Qed.
-  
-  Theorem e_update_same : forall x (m : Environment),
-      e_update m x (m x) = m.
+
+  Theorem e_update_same : forall x (m : Environment) v,
+    m ![x] = Some v ->
+      forall x', (e_update m x v) ![x'] = (m ![x']).
   Proof.
-    intros x m.
+    intros x m v HV x'.
     unfold e_update.
-    apply functional_extensionality.
-    intros x0.
-    case (plc_dec x x0).
-    * intros H; subst; reflexivity.
-    * intros H; reflexivity.
-  Qed.
+    map_unfold. unfold decEq_string.
+    destruct (plc_dec x' x); eauto.
+    subst. rewrite <- HV. refl.
+  Qed. 
 
   Theorem e_update_permute : forall v1 v2 x1 x2 (m : Environment),
       x2 <> x1 ->
-      (e_update (e_update m x2 v2) x1 v1)
-      = (e_update (e_update m x1 v1) x2 v2).
+      forall x', (e_update (e_update m x2 v2) x1 v1) ![x']
+      = ((e_update (e_update m x1 v1) x2 v2) ![x']).
   Proof.
-    intros v1 v2 x1 x2 m.
-    intros H.
+    intros v1 v2 x1 x2 m HX x'.
     unfold e_update.
-    apply functional_extensionality.
-    intros x.
-    case (plc_dec x1 x).
-    * intros H1. subst.
-      ** case (plc_dec x2 x); intros; contradiction || reflexivity.
-    * intros H1. subst.
-      ** case (plc_dec x2 x); intros; reflexivity.
+    map_unfold. unfold decEq_string.
+    destruct (plc_dec x' x2); eauto.
+    destruct (plc_dec x' x1); eauto.
+    cong.
   Qed.
 
   (** Definition of environments for use in examples and proofs.  Note they
@@ -124,100 +127,108 @@ Module ManifestTerm.
    *)
   Definition e0 := e_empty.
   Definition e1 :=
-    e_update e0 Rely (Some {| asps := [aspc1]; M:= [Target] |}).
+    (Rely !-> ({| asps := [aspc1]; M:= [Target] |}) ; e0).
   Definition e2 :=
-    e_update e1 Target (Some {| asps := [SIG]; M:= [Appraise] |}).
+    (Target !-> ({| asps := [SIG]; M:= [Appraise] |}) ; e1).
   Definition e3 :=
-    e_update e2 Appraise (Some {| asps := [HSH] ; M:= [] |}).
+    (Appraise !-> ({| asps := [HSH] ; M:= [] |}) ; e2).
   
   Inductive System : Type :=
   | env : Environment -> System
   | union : System -> System -> System.
 
 
-  Definition hasASPe(k:string)(e:Environment)(a:ASP):Prop :=
-    match (e k) with
-    | None => False
-    | Some m => In a m.(asps)
+  Definition hasASPe(k:string)(e:Environment)(a:ASP): bool :=
+    match (e ![k]) with
+    | None => false
+    | Some m => 
+      match in_dec asp_dec a m.(asps) with
+      | left _ => true
+      | right _ => false
+      end
     end.      
 
-  Fixpoint hasASPs(k:string)(s:System)(a:ASP):Prop :=
+  Fixpoint hasASPs(k:string)(s:System)(a:ASP): bool :=
     match s with
     | env e => (hasASPe k e a)
-    | union s1 s2 => (hasASPs k s1 a) \/ (hasASPs k s2 a)
+    | union s1 s2 => orb (hasASPs k s1 a) (hasASPs k s2 a)
     end.
 
-  (** Decidability of ASP presence should be true.  Hold for later
-  Theorem hasASP_dec: forall k e0 a, {hasASP k e0 a}+{~hasASP k e0 a}.
-   *)
-  
-  Example ex1: hasASPe Rely e3 aspc1.
-  Proof. unfold hasASPe. simpl. left. reflexivity. Qed.
+   Ltac prove_exec' :=
+    smp; eauto; unfold hasASPe; smp; 
+    destruct asp_dec; eauto; try cong.
+ 
+  Example ex1: hasASPe Rely e3 aspc1 = true.
+  Proof. prove_exec'. Qed.
 
-  Example ex2: hasASPe Rely e3 CPY -> False.
-  Proof. unfold hasASPe. simpl. intros. destruct H. inversion H. assumption. Qed.
+  Example ex2: hasASPe Rely e3 CPY = false.
+  Proof. prove_exec'. Qed.
   
-  Example ex5: hasASPs Rely (env e3) aspc1.
-  Proof. unfold hasASPs. unfold hasASPe. simpl. left. reflexivity. Qed.
+  Example ex5: hasASPs Rely (env e3) aspc1 = true.
+  Proof. prove_exec'. Qed.
 
-  Example ex6: hasASPs Rely (union (env e3) (env e2)) aspc1.
-  Proof. unfold hasASPs. left. unfold hasASPe. simpl. left. reflexivity. Qed.
+  Example ex6: hasASPs Rely (union (env e3) (env e2)) aspc1 = true.
+  Proof. prove_exec'. Qed.
 
   
   (** Determine if manifest [k] from [e] knows how to communicate from [k]
    * to [p]
    *)
-  Definition knowsOfe(k:string)(e:Environment)(p:Plc):Prop :=
-    match (e k) with
-    | None => False
-    | Some m => In p m.(M)
+  Definition knowsOfe(k:string)(e:Environment)(p:Plc): bool :=
+    match (e ![k]) with
+    | None => false
+    | Some m => 
+        match in_dec plc_dec p m.(M) with
+        | left _ => true
+        | right _ => false
+        end
     end.
 
-  Fixpoint knowsOfs(k:string)(s:System)(p:Plc):Prop :=
+  Fixpoint knowsOfs(k:string)(s:System)(p:Plc): bool :=
     match s with
     | env e => (knowsOfe k e p)
-    | union s1 s2 => (knowsOfs k s1 p) \/ (knowsOfs k s2 p)
+    | union s1 s2 => orb (knowsOfs k s1 p) (knowsOfs k s2 p)
     end.
 
-  Example ex3: knowsOfe Rely e3 Target.
+  Example ex3: knowsOfe Rely e3 Target = true.
   Proof.
-    unfold knowsOfe. simpl. auto.
+    prove_exec'.
   Qed.
   
-  Example ex4: knowsOfe Rely e3 Appraise -> False.
+  Example ex4: knowsOfe Rely e3 Appraise = false.
   Proof.
-    unfold knowsOfe. simpl. intros. destruct H. inversion H. assumption.
+    prove_exec'.
   Qed.
 
-  Example ex7: knowsOfs Rely (env e3) Target.
+  Example ex7: knowsOfs Rely (env e3) Target = true.
   Proof.
-    unfold knowsOfs,knowsOfe. simpl. auto.
+    prove_exec'.
   Qed.
 
-  Example ex8: knowsOfs Rely (union (env e3) (env e2)) Target.
+  Example ex8: knowsOfs Rely (union (env e3) (env e2)) Target = true.
   Proof.
-    unfold knowsOfs,knowsOfe. simpl. auto.
+    prove_exec'.
   Qed.
-  
+
   (** Is term [t] exectuable on the system described by manifest [k] in
    * manfiest map [e]?  Are the resources available?
    *)
-  Fixpoint executable(t:Term)(k:string)(e:Environment):Prop :=
+  Fixpoint executable(t:Term)(k:string)(e:Environment): bool :=
     match t with
     | asp a  => hasASPe k e a
-    | att p t => knowsOfe k e p /\ executable t p e
-    | lseq t1 t2 => executable t1 k e /\ executable t2 k e
-    | bseq _ t1 t2 => executable t1 k e /\ executable t2 k e
-    | bpar _ t1 t2 => executable t1 k e /\ executable t2 k e
+    | att p t => andb (knowsOfe k e p) (executable t p e)
+    | lseq t1 t2 => andb (executable t1 k e) (executable t2 k e)
+    | bseq _ t1 t2 => andb (executable t1 k e) (executable t2 k e)
+    | bpar _ t1 t2 => andb (executable t1 k e) (executable t2 k e)
     end.
 
-  Fixpoint executables(t:Term)(k:string)(s:System):Prop :=
+  Fixpoint executables(t:Term)(k:string)(s:System): bool :=
     match t with
     | asp a  => hasASPs k s a
-    | att p t => knowsOfs k s p /\ executables t p s
-    | lseq t1 t2 => executables t1 k s /\ executables t2 k s
-    | bseq _ t1 t2 => executables t1 k s /\ executables t2 k s
-    | bpar _ t1 t2 => executables t1 k s /\ executables t2 k s
+    | att p t => andb (knowsOfs k s p) (executables t p s)
+    | lseq t1 t2 => andb (executables t1 k s) (executables t2 k s)
+    | bseq _ t1 t2 => andb (executables t1 k s) (executables t2 k s)
+    | bpar _ t1 t2 => andb (executables t1 k s) (executables t2 k s)
     end.
 
   (** Proof tactic for proving [executable] given the above definition
@@ -232,27 +243,26 @@ Module ManifestTerm.
                  | |- ?A => idtac A
                  end.
 
-  Example ex9: (executable (asp SIG) Target e3).
-  Proof. prove_exec. Qed.
-  
-  Example ex10: (executable (asp CPY) Target e3) -> False.
+  Example ex9: (executable (asp SIG) Target e3) = true.
   Proof.
-    intros Hcontra.
-    simpl in *.
-    cbv in *.
-    destruct Hcontra.
-    discriminate. assumption.
+    prove_exec'.
+  Qed.
+  
+  Example ex10: (executable (asp CPY) Target e3) = false.
+  Proof.
+    prove_exec'.
   Qed.
 
-  Example ex11: (executable (lseq (asp SIG) (asp SIG)) Target e3).
-  Proof. prove_exec. Qed.
+  Example ex11: (executable (lseq (asp SIG) (asp SIG)) Target e3) = true.
+  Proof. prove_exec'. Qed.
 
   Example ex12: (executable (lseq (asp aspc1)
                               (att Target
                                  (lseq (asp SIG)
                                     (asp SIG))))
-                  Rely e3).
-  Proof. prove_exec. Qed.
+                  Rely e3) = true.
+  Proof. 
+    repeat prove_exec'. Qed.
 
   Ltac prove_execs :=
     simpl; auto; match goal with
@@ -270,10 +280,10 @@ Module ManifestTerm.
                                 (att Target
                                    (lseq (asp SIG)
                                       (asp SIG))))
-                  Rely (union (env e3) (env e2))).
-  Proof. prove_execs. Qed.
+                  Rely (union (env e3) (env e2))) = true.
+  Proof. repeat prove_exec'. Qed.
 
-
+(* 
   (* Experiments with classes. Nothing here.  Move along...*)
   Class Executable T P E :=
     { exec : T -> P -> E -> Prop }.
@@ -288,52 +298,51 @@ Module ManifestTerm.
   #[local]
   Instance sysExec: Executable Term string System :=
     { exec := executables
-    }.
+    }. *)
 
   (** Moving on to reasoning about system M *)
   
-  Definition R(e:Environment)(k1 k2:string):Prop :=
-    match (e k1) with
-    | Some m => In k2 m.(M)
-    | None => False
+  Definition R(e:Environment)(k1 k2:string): bool :=
+    match (e ![k1]) with
+    | Some m => 
+        match in_dec plc_dec k2 m.(M) with
+        | left _ => true
+        | right _ => false
+        end
+    | None => false
     end.
 
-  Example ex14: (R e3 Rely Target).
+  Example ex14: (R e3 Rely Target) = true.
   Proof. cbv. auto. Qed.
 
-  Example ex15: (R e3 Rely Appraise) -> False.
+  Example ex15: (R e3 Rely Appraise) = false.
   Proof.
-    prove_exec.
-    intros HContra.
-    cbv in *.
-    destruct HContra.
-    * inversion H.
-    * assumption.
+    refl.
   Qed.
   
-  Fixpoint Rs(s:System)(k1 k2:string):Prop :=
+  Fixpoint Rs(s:System)(k1 k2:string): bool :=
     match s with
     | env e => R e k1 k2
-    | union s1 s2 => Rs s1 k1 k2 \/ Rs s2 k1 k2
+    | union s1 s2 => orb (Rs s1 k1 k2) (Rs s2 k1 k2)
     end.
 
-  Example ex16: (Rs (env e3) Rely Target).
+  Example ex16: (Rs (env e3) Rely Target) = true.
   Proof.
     unfold Rs. apply ex14.
   Qed.
 
-  Example ex17: (Rs (union (env e3) (env e2)) Rely Target).
+  Example ex17: (Rs (union (env e3) (env e2)) Rely Target)= true.
   Proof.
-    unfold Rs. left. apply ex14.
+    unfold Rs. refl.
   Qed.
 
   (** Traces through [M]
    *)
   
-  Inductive trc {A} (R: A -> A -> Prop) : A -> A -> Prop :=
+  Inductive trc {A} (R: A -> A -> bool) : A -> A -> Prop :=
   | TrcRefl : forall x, trc R x x
   | TrcFront : forall x y z,
-    R x y
+    R x y = true
     -> trc R y z
     -> trc R x z.
 
@@ -346,23 +355,24 @@ Module ManifestTerm.
    *)
   Lemma ex19: (trc (R e3) Rely Appraise).
   Proof.
-    eapply TrcFront. constructor. reflexivity.
-    eapply TrcFront. constructor. reflexivity.
-    constructor.
+    unfold e3, e2, e1.
+    eapply (TrcFront (R e3) _ Target _). prove_exec.
+    eapply (TrcFront (R e3) _ Appraise _). prove_exec.
+    econstructor.
   Qed.
 
-  Inductive trcs {A} (Rs: A -> A -> Prop) : A -> A -> Prop :=
+  Inductive trcs {A} (Rs: A -> A -> bool) : A -> A -> Prop :=
   | TrcRefls : forall x, trcs Rs x x
   | TrcFronts : forall x y z,
-    Rs x y
+    Rs x y = true
     -> trcs Rs y z
     -> trcs Rs x z.
 
   Lemma ex20: (trcs (Rs (union (env e3) (env e2))) Rely Appraise).
   Proof.
-    eapply TrcFronts. constructor. unfold Rs. constructor. reflexivity.
-    eapply TrcFronts. constructor. unfold Rs. constructor. reflexivity.
-    eapply TrcRefls. 
+    eapply (TrcFronts (Rs (union (env e3) (env e2))) _ Target _). prove_exec.
+    eapply (TrcFronts (Rs (union (env e3) (env e2))) _ Appraise _). prove_exec.
+    econstructor.
   Qed.
 
 End ManifestTerm.
