src/Manifest/Ltacs.v
@@ -1,0 +1,37 @@
+Tactic Notation "smp" := (simpl in *).
+
+Ltac ind x := induction x.
+
+Ltac dest x := destruct x.
+
+Ltac refl := reflexivity.
+
+Ltac cong := congruence.
+
+(*
+  Inversion simpler notation tactics
+*)
+Ltac inv x := inversion x.
+Ltac invc x := inversion x; clear x.
+Ltac invsc x := inversion x; subst; clear x.
+
+(*
+  Print Goal - 
+    Helpful tactic when you want to see where something is failing
+    before restoring to original state
+*)
+(* Tactic Notation "PG" *)
+Ltac PG := match goal with |- ?A => idtac A end.
+
+(*
+  Solve_By_Inversion
+*)
+(* Tactic Notation "sbi" *)
+
+
+(*
+  Contradiction Solving
+*)
+Ltac qcon := 
+  (* TODO: Make more robust *)
+  intros C; try (inversion C || cong).
